vfmStateScript.sml
@@ -20,6 +20,10 @@ Definition wf_account_state_def:
   ∧ LENGTH a.code <= 2 ** 14 + 2 ** 13 (* https://eips.ethereum.org/EIPS/eip-170 *)
 End
 
-Type evm_accounts = “:address |-> account_state”
+Type evm_accounts = “:address -> account_state”
+
+Definition wf_accounts_def:
+  wf_accounts a ⇔ ∀x. wf_account_state (a x)
+End
 
 val _ = export_theory();
