vfmExecutionScript.sml
@@ -1,0 +1,19 @@
+open HolKernel boolLib bossLib Parse
+     vfmTypesTheory vfmContextTheory;
+
+val _ = new_theory"vfmExecution";
+
+Definition step_inst_def:
+  step_inst s i = s (* TODO *)
+End
+
+Definition step_def:
+  step s =
+  if s.contexts = [] then s else
+  let ctx = HD s.contexts in
+  let code = (s.accounts (ctx.callParams.callee)).code in
+  if ctx.pc ≥ LENGTH code then s else
+  step_inst s (EL ctx.pc code)
+End
+
+val _ = export_theory();
